sort

src/sorts.v
@@ -1,152 +1,160 @@
 Require Import Sorting.Permutation.
-Require Import List.
 Require Import Lia.
+Require Import List.
+Export ListNotations.
 Require Import Arith Arith.EqNat.
-Import ListNotations.
+Require Extraction.
 
+Fixpoint is_sorted' (l : list nat) : bool :=
+  match l with
+  | []      => true
+  | a :: l' => 
+      match l' with
+      | []       => true
+      | b :: l'' => leb a b && is_sorted' l'
+      end
+  end.
 
-
-(* Fixpoint is_sorted (l: list nat) :bool :=
-    match l with
-    | [] => true
-    | a :: l' => 
-        match l' with
-        | b :: l'' =>  leb a b && is_sorted l'
-        | [] => true
-        end
-    end. *)
-   
 Inductive is_smallest : nat -> list nat -> Prop :=
 | smallest_unit : forall a, is_smallest a [a]
-| smallest_head : forall a b tl 
-                    (LE : a <= b)
-                    (SST: is_smallest b tl),
-                is_smallest a (a :: tl)    
-| smallest_tail : forall a b tl 
-                    (LE : a <= b)
-                    (SST: is_smallest a tl),
-                is_smallest a (b :: tl)
+| smallest_head : forall a b tl
+                         (LE  : a <= b)
+                         (SST : is_smallest b tl),
+    is_smallest a (a :: tl)
+| smallest_tail : forall a b tl
+                         (LT : a < b)
+                         (SST : is_smallest a tl),
+    is_smallest a (b :: tl)
 .
 
 Inductive is_sorted : list nat -> Prop :=
-| sorted_nil  : is_sorted []
-| sorted_one  : forall a, is_sorted [a] 
-| sorted_cons : forall a tl 
-                    (SORTED : is_sorted tl) 
-                    (SST    : is_smallest a (a :: tl)), 
-                is_sorted (a :: tl)
-
+| sorted_nil   : is_sorted []
+| sorted_one a : is_sorted [a]
+| sorted_cons a tl
+              (SORTED : is_sorted tl)
+              (SST : is_smallest
+                       a (a :: tl))
+  :
+    is_sorted (a :: tl)
 .
 
+Theorem sort l :
+  { l' | Permutation l l' & is_sorted l' }.
+Proof.
+  induction l.
+  { exists [].
+    { apply perm_nil. }
+    apply sorted_nil. }
+  inversion IHl.
+  rename x into l'.
+  rename H into PERM.
+  rename H0 into SORT.
+Abort.
 
 Inductive is_inserted : nat -> list nat -> list nat -> Prop
-    :=
+  :=
 | ins_head : forall n tl, is_inserted n tl (n :: tl)
-| ins_tail : forall n m tl tl' (INS : is_inserted n tl tl'),
-                is_inserted n (m :: tl) (m :: tl')
+| ins_tail : forall n m tl tl'
+                    (INS : is_inserted n tl tl'),
+    is_inserted n (m :: tl) (m :: tl')
 .
 
-Lemma is_inserted_perm a tl tl' (INS : is_inserted a tl tl') :
-Permutation (a :: tl) tl'.
+Lemma is_inserted_perm a tl tl' 
+  (INS : is_inserted a tl tl') :
+  Permutation (a :: tl) tl'.
 Proof.
-    generalize dependent a.
-    generalize dependent tl'.
-    induction tl.
-    {   intros.
-        inversion INS. 
-        apply Permutation_refl.    }
-    intros.
-    inversion INS.
-    { apply Permutation_refl. }
-    apply IHtl in INS0.
-    (* apply perm_trans with (l' := (a :: a0 :: tl)). *)
-    eapply perm_trans.
-    { apply perm_swap. }
-    apply perm_skip.
-    apply INS0.
+  generalize dependent a.
+  generalize dependent tl'.
+  induction tl.
+  { intros.
+    inversion INS.  
+    apply Permutation_refl. }
+    (* Search Permutation. *)
+    (* apply perm_skip. *)
+    (* apply perm_nil. *)
+  intros.
+  inversion INS.
+  { apply Permutation_refl. }
+  apply IHtl in INS0.
+  (* apply perm_trans with (l' := (a :: a0 :: tl)). *)
+  eapply perm_trans.
+  { apply perm_swap. }
+  apply perm_skip. apply INS0.
 Qed.
 
-Lemma insert_sorted a l (SORT: is_sorted l) : 
-{ l' | is_inserted a l l' & is_sorted l'}.
-Proof. Admitted.
-    (* induction l.
-    {exists [a]; constructor. }
-    assert ( is_sorted l) as AA.
-    { inversion SORT. 
-        {constructor. }
-        assumption. }
-    apply IHl in AA.
-    clear IHl.
-    destruct AA as [l' INS SORT'].
-    
-    destruct (le_gt_dec a a0) as [AA|AA].
-    { exists (a :: a0 :: l). 
-        { constructor. }
-        constructor. 
-        { auto. }
-        eapply smallest_head.
-        { apply AA. }
-        inversion SORT.
-        { constructor. }
-        assumption. }
-    exists (a0 :: l').
-    { constructor. auto. }
-    inversion SORT.
-    { subst. 
-    inversion INS. 
-    subst. 
-    constructor.
+Lemma insert_sorted a l (SORT : is_sorted l) :
+  { l' | is_inserted a l l' & is_sorted l'}.
+Proof.
+  induction l.
+  { exists [a]; constructor. }
+  edestruct IHl as [l'].
+  { clear -SORT. inversion SORT; subst.
     { constructor. }
-    eapply smallest_head.
-    2: constructor.
-    lia. }
-    subst.
-    clear SORT SORTED.
-    constructor.
-    { assumption. }
-    clear SORT'.
-    
-    generalize dependent l'.
-    generalize dependent a.
+    assumption. }
+  destruct (le_gt_dec a a0).
+  { exists (a::a0::l).
+    { constructor. }
+    apply sorted_cons; auto.
+    eapply smallest_head; eauto.
+    inversion SORT; subst.
+    { constructor. }
+    assumption. }
 
-    induction l; intros.
-    { inversion INS. subst.
-     eapply smallest_head.
-     2: constructor.
-     lia. }
+  exists (a0::l').
+  { constructor. assumption. }
+  
+  clear -SORT i i0 g.
+  induction i. 
+  { constructor; auto.
+    eapply smallest_head with (b:=n).
+    { lia. }
+    inversion i0; subst.
+    { constructor. }
+    assumption. }
 
-    assert (is_smallest a0 (a0 :: l)) as BB.
-    { inversion SST; subst. }. Admitted. *)
-    
-        
-    
-    
-    
+  constructor; auto.
+  apply smallest_head with (b:=m).
+  2: { inversion i0; subst.
+       { constructor. }
+       assumption. }
+  
+  clear -SORT.
+  inversion SORT; subst.
+  inversion SST; subst.
+  2: lia.
+  inversion SST0; subst.
+  { assumption. }
+  { assumption. }
+  lia.
+Defined.
 
-
-
-
-
-Theorem  sort l: 
-    { l' | Permutation l l' & is_sorted l'}
-.
+Theorem sort l :
+  { l' | Permutation l l' & is_sorted l' }.
 Proof.
-    induction l.
-    { exists [].
-    {apply perm_nil. }
-    apply sorted_nil.
-    }
-    inversion IHl.
-    rename x into l'.
-    rename H into PERM.
-    rename H0 into SORT.
-    apply (insert_sorted a l') in  SORT.
-    destruct SORT as [l'' AA BB].
-    exists l''.
-    2: apply BB.
-    apply is_inserted_perm in AA. 
-    eapply perm_trans. 
-    2: apply AA. 
-    apply perm_skip. 
-    apply PERM.  
-Qed.
+  induction l.
+  { exists [].
+    { apply perm_nil. }
+    apply sorted_nil. }
+  inversion IHl.
+  rename x into l'.
+  rename H into PERM.
+  rename H0 into SORT.
+  apply (insert_sorted a l') in SORT.
+  destruct SORT as [l'' AA BB].
+  exists l''.
+  2: { apply BB. }
+  apply is_inserted_perm in AA.
+  eapply perm_trans.
+  2: apply AA.
+  apply perm_skip.
+  apply PERM.
+Defined.
+
+Print sort.
+
+Extraction Language OCaml.
+
+
+
+
+
